examples/cannon/CannonMainIAproof.v
@@ -12,19 +12,18 @@ Module CannonMainIA. Section CannonMainIA.
   Context `{!invG α Σ Γ, !subG Γ Σ, !sinvG Σ Γ α β τ}.
   Context `{!CannonAGΓ Γ}.
 
-  Context (u_s: univ_id).
   Context (SpcMain : string → option fspec).
   Context (CannonInMain : spc_incl CannonAS.Spc SpcMain).
 
   Definition Ist : nat → alist key Any.t → alist key Any.t → iProp Σ :=
     λ _ _ _, (True)%I.
 
-  Local Definition MainAMod := (MainA.t 1 u_s SpcMain).
+  Local Definition MainAMod := (MainA.t 1 SpcMain).
   Local Definition MainIMod := (MainI.t 1).
   
   Lemma simF_main : HSim.sim_fun open MainAMod MainIMod Ist MainName.main.
   Proof.
-    winit_simF u_s 0.
+    winit_simF 0 0.
     wsteps_l. iDestruct "ASM" as "((%Y & B) & %Q)". subst. hss.
     wsteps_r. 
     unfold HoareCall. wforce_l. instantiate (1:=()). wforce_l.
@@ -43,15 +42,15 @@ Module CannonMainIA. Section CannonMainIA.
   Qed.
 End CannonMainIA.
 
-Section wctxr.
+Section ctxr.
   Context `{!invG α Σ Γ, !subG Γ Σ, !sinvG Σ Γ α β τ}.
   Context `{!CannonAGΓ Γ}.
 
-  Theorem wctxr (u: univ_id) (SpcMain : string → option fspec)
+  Theorem ctxr (SpcMain : string → option fspec)
     (CannonInMain : spc_incl CannonAS.Spc SpcMain)
   :
     ctx_refines
-      (MainA.t 1 u SpcMain, (MainA.init_cond))
+      (MainA.t 1 SpcMain, (MainA.init_cond))
       (MainI.t 1, (emp%I)).
   Proof. eapply main_adequacy, sim; eauto. Qed.
-End wctxr. End CannonMainIA.
+End ctxr. End CannonMainIA.
