examples/incr/IncrHeader.v
@@ -1,5 +1,0 @@
-(* Require Import CRIS.
-
-Module IncrName.
-  Definition incr := "Incr.incr".
-End IncrName. *)
