examples/incr/IncrMainI.v
@@ -8,36 +8,26 @@ Module IncrMainI. Section IncrMainI.
 
   Definition main : unit → itree pmodE unit :=
     λ _,
-      Sch.yield;;;
-      'ptr_raw : val <- ccallU MemName.alloc [Vint 1%Z];;
-      '(blk, ofs) : mblock * ptrofs <- (pargs [Tptr] [ptr_raw])?;;
-      Sch.yield;;;
-      '_ : val <- ccallU MemName.store [Vptr blk ofs; Vint 0%Z];;
-      Sch.yield;;;
-      tid1 <- Sch.spawn ("f", [Vptr blk ofs]↑↑);;
-      Sch.yield;;;
-      tid2 <- Sch.spawn ("f", [Vptr blk ofs]↑↑);;
-      Sch.yield;;;
-      Sch.join unit tid1;;;
-      Sch.yield;;;
-      Sch.join unit tid2;;;
-      Sch.yield;;;
-      'v_raw : val <- ccallU MemName.load [Vptr blk ofs];;
-      'v : Z <- (pargs [Tint] [v_raw])?;;
-      Sch.yield;;;
-      '_ : unit <- trigger (IO "OUT" v);;
-      Sch.yield;;;
-      Ret tt.
+      𝒴;;; 'ptr_raw : val <- ccallU MemName.alloc [Vint 1%Z];;
+      𝒴;;; '(blk, ofs) : mblock * ptrofs <- (pargs [Tptr] [ptr_raw])?;;
+      𝒴;;; '_ : val <- ccallU MemName.store [Vptr blk ofs; Vint 0%Z];;
+      𝒴;;; tid1 <- Sch.spawn ("f", [Vptr blk ofs]↑↑);;
+      𝒴;;; tid2 <- Sch.spawn ("f", [Vptr blk ofs]↑↑);;
+      𝒴;;; Sch.join tid1;;;
+      𝒴;;; Sch.join tid2;;;
+      𝒴;;; 'v_raw : val <- ccallU MemName.load [Vptr blk ofs];;
+      𝒴;;; 'v : Z <- (pargs [Tint] [v_raw])?;;
+      𝒴;;; '_ : unit <- trigger (IO "OUT" v);;
+      𝒴;;; Ret tt.
   
   Definition f : list val → itree pmodE unit :=
     λ arg,
-      '(blk, ofs) : mblock * ptrofs <- (pargs [Tptr] arg)?;;
-      Sch.yield;;;
-      'v_raw : val <- ccallU MemName.load [Vptr blk ofs];;
-      'v : Z <- (pargs [Tint] [v_raw])?;;
-      '_ : val <- ccallU MemName.store [Vptr blk ofs; Vint (v + 1)%Z];;
-      Sch.yield;;;
-      Ret tt.
+      𝒴;;; '(blk, ofs) : mblock * ptrofs <- (pargs [Tptr] arg)?;;
+      (* atomic update *)
+      𝒴;;; 'v_raw : val <- ccallU MemName.load [Vptr blk ofs];;
+            'v : Z <- (pargs [Tint] [v_raw])?;;
+            '_ : val <- ccallU MemName.store [Vptr blk ofs; Vint (v + 1)%Z];;
+      𝒴;;; Ret tt.
 
   Definition fnsems :=
     [(MainName.main, (scopes, cfunU main));
