examples/mutsum/MutAll.v
@@ -51,7 +51,7 @@ Module MutAll.
     etrans. { eapply ctxr_comm. }
     etrans.
     { rewrite -hmod_addc_empty_l. eapply ctxr_cond_frameR.
-      replace (SMod.to_hmod ginv spc APCC.Mod) with (APCC.t 1 spc); cycle 1.
+      replace (SMod.to_hmod ginv spc APCC.Mod) with (APCC.t u spc); cycle 1.
       { unfold APCC.t. unseal CRIS. ss. }
       eapply APCAC.wctxr.
       { instantiate (1:=spc). prove_spc. }
@@ -62,13 +62,13 @@ Module MutAll.
     rewrite !hmod_add_assoc. rewrite -(hmod_add_assoc (SMod.to_hmod ginv spc MutFA.Mod)).
     etrans.
     { eapply ctxr_compose_mix.
-      { replace (SMod.to_hmod ginv spc MutMainA.Mod) with (MutMainA.t 1 spc); cycle 1.
+      { replace (SMod.to_hmod ginv spc MutMainA.Mod) with (MutMainA.t u spc); cycle 1.
         { unfold MutMainA.t. unseal CRIS. ss. }
         eapply MutMainIA.wctxr; prove_spc.
       }
-      { replace (SMod.to_hmod ginv spc MutFA.Mod) with (MutFA.t 1 spc); cycle 1.
+      { replace (SMod.to_hmod ginv spc MutFA.Mod) with (MutFA.t u spc); cycle 1.
         { unfold MutFA.t. unseal CRIS. ss. }
-        replace (SMod.to_hmod ginv spc MutGA.Mod) with (MutGA.t 1 spc); cycle 1.
+        replace (SMod.to_hmod ginv spc MutGA.Mod) with (MutGA.t u spc); cycle 1.
         { unfold MutGA.t. unseal CRIS. ss. }
         rewrite !hmod_add_assoc.
         etrans.
